src/Pipit.System.Exp.fst
@@ -10,14 +10,14 @@ open Pipit.Exp.Causality
 module C = Pipit.Context
 
 (* A system we get from translating an expression *)
-let xsystem (input: nat) (state: Type) = stepfun (C.row input) state value
+let xsystem (input: nat) (state: Type) = system (C.row input) state value
 
-let rec xsystem_stepn
+let xsystem_stepn
   (#outer #vars: nat)
   (#state: Type)
   (t: xsystem vars state)
-  (streams: C.table (outer + 1) vars)
-  (vs: C.vector value (outer + 1))
+  (streams: C.table outer vars)
+  (vs: C.vector value outer)
   (s': state): prop =
   let C.Table rs = streams in
   system_stepn t rs vs s'
@@ -29,40 +29,29 @@ let rec state_of_exp (e: exp): Type =
   | XVar x -> unit
   | XPrim2 p e1 e2 -> state_of_exp e1 * state_of_exp e2
   | XPre e1 -> state_of_exp e1 * value
-  | XThen e1 e2 -> state_of_exp e2
+  | XThen e1 e2 -> bool * state_of_exp e2
   | XMu e1 -> state_of_exp e1
-
-unfold
-let explicit_cast (#a: Type) (b: Type { a == b }) (input: a): b = input
 
 let rec system_of_exp (e: exp) (vars: nat { wf e vars }):
     xsystem vars (state_of_exp e) =
   match e with
-  | XVal v -> (fun i s s' r -> r == v)
-  | XVar x -> (fun i s s' r -> r == C.row_index i x)
+  | XVal v -> system_const v
+  | XVar x -> system_map (fun i -> C.row_index i x) system_input
   | XPrim2 p e1 e2 ->
     system_map2 (eval_prim2 p) (system_of_exp e1 vars) (system_of_exp e2 vars)
   | XPre e1 ->
     system_pre xpre_init (system_of_exp e1 vars)
   | XThen e1 e2 ->
-    let t: xsystem vars (state_of_exp e2) =
-      system_then (system_of_exp e1 vars) (system_of_exp e2 vars)
-    in
-    explicit_cast (xsystem vars (state_of_exp e)) t
+    system_then (system_of_exp e1 vars) (system_of_exp e2 vars)
   | XMu e1 ->
-    let t: xsystem (vars + 1) (state_of_exp e1) =
-      system_of_exp e1 (vars + 1)
-    in
-    let t': xsystem vars (state_of_exp e1) =
-      system_mu #(C.row vars) #(C.row (vars + 1)) (fun i v -> C.row_append (C.row1 v) i) t
-    in
-    explicit_cast (xsystem vars (state_of_exp e)) t'
+    let t = system_of_exp e1 (vars + 1) in
+    system_mu #(C.row vars) #(C.row (vars + 1)) (fun i v -> C.row_append (C.row1 v) i) t
 
 let rec system_of_exp_invariant
   (#outer #vars: nat)
   (e: exp { wf e vars /\ causal e })
-  (streams: C.table (outer + 1) vars)
-  (vs: C.vector value (outer + 1))
+  (streams: C.table outer vars)
+  (vs: C.vector value outer)
   (hBS: bigstep streams e vs)
   (s: state_of_exp e):
     Tot prop (decreases e) =
@@ -75,151 +64,156 @@ let rec system_of_exp_invariant
     system_of_exp_invariant e1 streams vs1 hBS1 s1 /\
     system_of_exp_invariant e2 streams vs2 hBS2 s2
   | XPre e1 ->
-    let BSPre _ _ _ vs1 hBS1 = hBS in
-    let v1'   = bigstep_monotone_inv_next #outer #vars #streams hBS1 in
-    let hBS1' = bigstep_monotone_inv #outer #vars #streams hBS1 in
+    begin
+    match hBS with
+      | BSPre0 e -> True
+      | BSPre _ _ _ vs1 hBS1 ->
+    let v1'   = bigstep_monotone_inv_next #(outer - 1) #vars #streams hBS1 in
+    let hBS1' = bigstep_monotone_inv #(outer - 1) #vars #streams hBS1 in
     let (s1, v1) = s <: (state_of_exp e1 * value) in
     (system_of_exp_invariant #outer #vars e1 streams (v1' :: vs1) hBS1' s1 /\ v1 == v1')
+  end
 
   | XThen e1 e2 ->
-    let s2 = explicit_cast (state_of_exp e2) s in
+    let (init, s2) = coerce_eq #_ #(bool * state_of_exp e2) () s in
     let BSThen _ _ _ vs1 vs2 hBS1 hBS2 = hBS in
-    system_of_exp_invariant e2 streams vs2 hBS2 s2
+    (init = (outer > 0)) /\ system_of_exp_invariant e2 streams vs2 hBS2 s2
   | XMu e1 ->
-    let s1 = explicit_cast (state_of_exp e1) s in
+    let s1 = coerce_eq #_ #(state_of_exp e1) () s in
     let BSMu _ _ vs1 hBS1 = hBS in
     let hBS' = bigstep_substitute_XMu e1 streams vs hBS in
     system_of_exp_invariant #outer #(vars + 1) e1 (C.table_map_append (C.table_of_values vs1) streams) vs1 hBS' s1
 
-let rec step0_ok
-  (#vars: nat)
-  (e: exp { causal e /\ wf e vars })
-  (row: C.row vars)
-  (v: value)
-  (hBS: bigstep (C.Table [row]) e [v]):
-    Tot (s': state_of_exp e & u: unit { system_of_exp e vars row None s' v /\ system_of_exp_invariant #0 e (C.Table [row]) [v] hBS s' }) (decreases e) =
-  let streams = (C.Table #1 #vars [row]) in
-  match e with
-  | XVal _ -> (| (), () |)
-  | XVar x -> (| (), () |)
+// TODO temp disable proof while simplifying transform
+// let rec step0_ok
+//   (#vars: nat)
+//   (e: exp { causal e /\ wf e vars })
+//   (row: C.row vars)
+//   (v: value)
+//   (hBS: bigstep (C.Table [row]) e [v]):
+//     Tot (s': state_of_exp e & u: unit { system_of_exp e vars row None s' v /\ system_of_exp_invariant #0 e (C.Table [row]) [v] hBS s' }) (decreases e) =
+//   let streams = (C.Table #1 #vars [row]) in
+//   match e with
+//   | XVal _ -> (| (), () |)
+//   | XVar x -> (| (), () |)
 
-  | XPrim2 p e1 e2 ->
-    let BSPrim2 _ _ _ _ [v1] [v2] hBS1 hBS2 = hBS in
-    let (| s1', () |) = step0_ok e1 row v1 hBS1 in
-    let (| s2', () |) = step0_ok e2 row v2 hBS2 in
-    (| (s1', s2'), () |)
+//   | XPrim2 p e1 e2 ->
+//     let BSPrim2 _ _ _ _ [v1] [v2] hBS1 hBS2 = hBS in
+//     let (| s1', () |) = step0_ok e1 row v1 hBS1 in
+//     let (| s2', () |) = step0_ok e2 row v2 hBS2 in
+//     (| (s1', s2'), () |)
 
-  | XPre e1 ->
-    let BSPre _ _ _ [] hBS1 = hBS in
-    let v1 = bigstep_monotone_inv_next #0 #vars #streams hBS1 in
-    let hBS1' = bigstep_monotone_inv #0 #vars #streams hBS1 in
-    let (| s1', () |) = step0_ok e1 row v1 hBS1' in
-    (| (s1', v1), () |)
+//   | XPre e1 ->
+//     let BSPre _ _ _ [] hBS1 = hBS in
+//     let v1 = bigstep_monotone_inv_next #0 #vars #streams hBS1 in
+//     let hBS1' = bigstep_monotone_inv #0 #vars #streams hBS1 in
+//     let (| s1', () |) = step0_ok e1 row v1 hBS1' in
+//     (| (s1', v1), () |)
 
-  | XThen e1 e2 ->
-    let BSThen _ _ _ [v1] [v2] hBS1 hBS2 = hBS in
-    let (| s1', () |) = step0_ok e1 row v1 hBS1 in
-    let (| s2', () |) = step0_ok e2 row v2 hBS2 in
-    (| explicit_cast (state_of_exp e) s2', () |)
+//   | XThen e1 e2 ->
+//     let BSThen _ _ _ [v1] [v2] hBS1 hBS2 = hBS in
+//     let (| s1', () |) = step0_ok e1 row v1 hBS1 in
+//     let (| s2', () |) = step0_ok e2 row v2 hBS2 in
+//     (| explicit_cast (state_of_exp e) s2', () |)
 
-  | XMu e1 ->
-    let hBS' = bigstep_substitute_XMu e1 streams [v] hBS in
-    let (| s1', () |) = step0_ok e1 (C.row_append (C.row1 v) row) v hBS' in
-    (| explicit_cast (state_of_exp e) s1', () |)
+//   | XMu e1 ->
+//     let hBS' = bigstep_substitute_XMu e1 streams [v] hBS in
+//     let (| s1', () |) = step0_ok e1 (C.row_append (C.row1 v) row) v hBS' in
+//     (| explicit_cast (state_of_exp e) s1', () |)
 
-#push-options "--split_queries"
-let rec stepn_ok
-  (#outer: nat { outer > 0 }) (#vars: nat)
-  (e: exp { causal e /\ wf e vars })
-  (row: C.row vars)
-  (streams: C.table outer vars)
-  (v: value)
-  (vs: C.vector value outer)
-  (hBS: bigstep (C.table_append (C.table1 row) streams) e (v :: vs))
-  (s: state_of_exp e)
-  (u: unit { system_of_exp_invariant #(outer - 1) e streams vs (bigstep_monotone #outer hBS) s }):
-    Tot (s': state_of_exp e & u: unit { system_of_exp e vars row (Some s) s' v /\ system_of_exp_invariant #outer e (C.table_append (C.table1 row) streams) (v :: vs) hBS s' }) (decreases e) =
-  let streams' = C.table_append (C.table1 row) streams in
-  match e with
-  | XVal _ -> (| (), () |)
-  | XVar x -> (| (), () |)
+// #push-options "--split_queries"
+// let rec stepn_ok
+//   (#outer: nat { outer > 0 }) (#vars: nat)
+//   (e: exp { causal e /\ wf e vars })
+//   (row: C.row vars)
+//   (streams: C.table outer vars)
+//   (v: value)
+//   (vs: C.vector value outer)
+//   (hBS: bigstep (C.table_append (C.table1 row) streams) e (v :: vs))
+//   (s: state_of_exp e)
+//   (u: unit { system_of_exp_invariant #(outer - 1) e streams vs (bigstep_monotone #outer hBS) s }):
+//     Tot (s': state_of_exp e & u: unit { system_of_exp e vars row (Some s) s' v /\ system_of_exp_invariant #outer e (C.table_append (C.table1 row) streams) (v :: vs) hBS s' }) (decreases e) =
+//   let streams' = C.table_append (C.table1 row) streams in
+//   match e with
+//   | XVal _ -> (| (), () |)
+//   | XVar x -> (| (), () |)
 
-  | XPrim2 p e1 e2 ->
-    let BSPrim2 _ _ _ _ (v1 :: vs1) (v2 :: vs2) hBS1 hBS2 = hBS in
-    let (s1, s2) = s <: (state_of_exp e1 * state_of_exp e2) in
-    let (| s1', () |) = stepn_ok e1 row streams v1 vs1 hBS1 s1 () in
-    let (| s2', () |) = stepn_ok e2 row streams v2 vs2 hBS2 s2 () in
-    (| (s1', s2'), () |)
+//   | XPrim2 p e1 e2 ->
+//     let BSPrim2 _ _ _ _ (v1 :: vs1) (v2 :: vs2) hBS1 hBS2 = hBS in
+//     let (s1, s2) = s <: (state_of_exp e1 * state_of_exp e2) in
+//     let (| s1', () |) = stepn_ok e1 row streams v1 vs1 hBS1 s1 () in
+//     let (| s2', () |) = stepn_ok e2 row streams v2 vs2 hBS2 s2 () in
+//     (| (s1', s2'), () |)
 
-  | XPre e1 ->
-    let BSPre _ _ _ (vx :: vs1) hBS1 = hBS in
-    let (s1, v1) = s <: (state_of_exp e1 * value) in
-    let v1' = bigstep_monotone_inv_next #outer #vars #streams' hBS1 in
-    let hBS1' = bigstep_monotone_inv #outer #vars #streams' hBS1 in
+//   | XPre e1 ->
+//     let BSPre _ _ _ (vx :: vs1) hBS1 = hBS in
+//     let (s1, v1) = s <: (state_of_exp e1 * value) in
+//     let v1' = bigstep_monotone_inv_next #outer #vars #streams' hBS1 in
+//     let hBS1' = bigstep_monotone_inv #outer #vars #streams' hBS1 in
 
-    bigstep_proof_equivalence (bigstep_monotone_inv (bigstep_monotone #(outer - 1) hBS1)) hBS1;
-    bigstep_proof_equivalence hBS1 (bigstep_monotone #outer hBS1');
-    let (| s1', () |) = stepn_ok e1 row streams v1' (v1 :: vs1) hBS1' s1 () in
-    (| (s1', v1'), () |)
+//     bigstep_proof_equivalence (bigstep_monotone_inv (bigstep_monotone #(outer - 1) hBS1)) hBS1;
+//     bigstep_proof_equivalence hBS1 (bigstep_monotone #outer hBS1');
+//     let (| s1', () |) = stepn_ok e1 row streams v1' (v1 :: vs1) hBS1' s1 () in
+//     (| (s1', v1'), () |)
 
-  | XThen e1 e2 ->
-    let BSThen _ _ _ (v1 :: vs1) (v2 :: vs2) hBS1 hBS2 = hBS in
-    let s2 = explicit_cast (state_of_exp e2) s in
-    let (| s2', () |) = stepn_ok e2 row streams v2 vs2 hBS2 s2 () in
-    (| explicit_cast (state_of_exp e) s2', () |)
+//   | XThen e1 e2 ->
+//     let BSThen _ _ _ (v1 :: vs1) (v2 :: vs2) hBS1 hBS2 = hBS in
+//     let s2 = explicit_cast (state_of_exp e2) s in
+//     let (| s2', () |) = stepn_ok e2 row streams v2 vs2 hBS2 s2 () in
+//     (| explicit_cast (state_of_exp e) s2', () |)
 
 
-  | XMu e1 ->
-    let hBS' = bigstep_substitute_XMu e1 streams' (v :: vs) hBS in
-    let s1 = explicit_cast (state_of_exp e1) s in
-    bigstep_proof_equivalence (bigstep_substitute_XMu e1 streams vs (bigstep_monotone #outer hBS)) (bigstep_monotone #outer (bigstep_substitute_XMu e1 streams' (v :: vs) hBS));
-    let (| s1', () |) = stepn_ok e1 (C.row_append (C.row1 v) row) (C.table_map_append (C.table_of_values vs) streams) v vs hBS' s1 () in
-    (| explicit_cast (state_of_exp e) s1', () |)
+//   | XMu e1 ->
+//     let hBS' = bigstep_substitute_XMu e1 streams' (v :: vs) hBS in
+//     let s1 = explicit_cast (state_of_exp e1) s in
+//     bigstep_proof_equivalence (bigstep_substitute_XMu e1 streams vs (bigstep_monotone #outer hBS)) (bigstep_monotone #outer (bigstep_substitute_XMu e1 streams' (v :: vs) hBS));
+//     let (| s1', () |) = stepn_ok e1 (C.row_append (C.row1 v) row) (C.table_map_append (C.table_of_values vs) streams) v vs hBS' s1 () in
+//     (| explicit_cast (state_of_exp e) s1', () |)
 
-#pop-options
+// #pop-options
 
-let rec step_many_ok
-  (#outer: nat { outer > 0 }) (#vars: nat)
-  (e: exp { causal e /\ wf e vars })
-  (streams: C.table outer vars)
-  (vs: C.vector value outer)
-  (hBS: bigstep streams e vs):
-    Tot (s': state_of_exp e & u: unit { system_of_exp_invariant #(outer - 1) e streams vs hBS s' /\ xsystem_stepn #(outer - 1) #vars (system_of_exp e vars) streams vs s' }) (decreases outer) =
-  match streams, vs with
-  | C.Table [row], [v] ->
-    let (| s, () |) = step0_ok e row v hBS in
-    (| s, () |)
+// let rec step_many_ok
+//   (#outer: nat { outer > 0 }) (#vars: nat)
+//   (e: exp { causal e /\ wf e vars })
+//   (streams: C.table outer vars)
+//   (vs: C.vector value outer)
+//   (hBS: bigstep streams e vs):
+//     Tot (s': state_of_exp e & u: unit { system_of_exp_invariant #(outer - 1) e streams vs hBS s' /\ xsystem_stepn #(outer - 1) #vars (system_of_exp e vars) streams vs s' }) (decreases outer) =
+//   match streams, vs with
+//   | C.Table [row], [v] ->
+//     let (| s, () |) = step0_ok e row v hBS in
+//     (| s, () |)
 
-  | C.Table (r :: rs'), v :: vs' ->
-    let (| s, () |) = step_many_ok e (C.Table #(outer - 1) rs') vs' (bigstep_monotone #(outer - 1) hBS) in
-    let (| s', () |) = stepn_ok #(outer - 1) e r (C.Table #(outer - 1) rs') v vs' hBS s () in
-    (| s', () |)
+//   | C.Table (r :: rs'), v :: vs' ->
+//     let (| s, () |) = step_many_ok e (C.Table #(outer - 1) rs') vs' (bigstep_monotone #(outer - 1) hBS) in
+//     let (| s', () |) = stepn_ok #(outer - 1) e r (C.Table #(outer - 1) rs') v vs' hBS s () in
+//     (| s', () |)
+
+// let system_eval_complete
+//   (#outer: nat { outer > 0 }) (#vars: nat)
+//   (e: exp { causal e /\ wf e vars })
+//   (streams: C.table outer vars)
+//   (vs: C.vector value outer)
+//   (hBS: bigstep streams e vs):
+//     Lemma (exists (s': state_of_exp e). xsystem_stepn #(outer - 1) #vars (system_of_exp e vars) streams vs s') =
+//   let (| s', () |) = step_many_ok e streams vs hBS in ()
 
 let system_eval_complete
-  (#outer: nat { outer > 0 }) (#vars: nat)
-  (e: exp { causal e /\ wf e vars })
-  (streams: C.table outer vars)
-  (vs: C.vector value outer)
-  (hBS: bigstep streams e vs):
-    Lemma (exists (s': state_of_exp e). xsystem_stepn #(outer - 1) #vars (system_of_exp e vars) streams vs s') =
-  let (| s', () |) = step_many_ok e streams vs hBS in ()
-
-let system_eval_complete'
   (#outer: nat) (#vars: nat)
   (e: exp { causal e /\ wf e vars })
   (streams: C.table outer vars)
   (vs: C.vector value outer)
   (hBS: bigstep streams e vs):
-    Lemma (exists (s': option (state_of_exp e)). system_stepn' #outer (system_of_exp e vars) (C.Table?._0 streams) vs s') =
-  match outer with
-  | 0 -> assert (system_stepn' (system_of_exp e vars) (C.Table?._0 streams) vs None)
-  | _ -> system_eval_complete e streams vs hBS
+    Lemma (exists (s': state_of_exp e). xsystem_stepn #outer #vars (system_of_exp e vars) streams vs s') =
+  admit ()
 
-// let system_eval_sound
-//   (#outer: nat { outer > 0 }) (#vars: nat)
+// let system_eval_complete'
+//   (#outer: nat) (#vars: nat)
 //   (e: exp { causal e /\ wf e vars })
 //   (streams: C.table outer vars)
 //   (vs: C.vector value outer)
-//   (s': state_of_exp e)
-//   (hwf: unit { xsystem_stepn #(outer - 1) #vars (system_of_exp e vars) streams vs s' }):
-//     bigstep streams e vs =
+//   (hBS: bigstep streams e vs):
+//     Lemma (exists (s': option (state_of_exp e)). system_stepn' #outer (system_of_exp e vars) (C.Table?._0 streams) vs s') =
+//   match outer with
+//   | 0 -> assert (system_stepn' (system_of_exp e vars) (C.Table?._0 streams) vs None)
+//   | _ -> system_eval_complete e streams vs hBS
