src/Pipit.System.Ind.fst
@@ -9,43 +9,60 @@ let rec prop_for_all (l: list prop): prop =
  | [] -> True
  | p :: ps -> p /\ prop_for_all ps
 
-let base_case (#input #state: Type) (t: stepfun input state prop): prop =
-  forall (i: input) (s': state) (r: prop).
-    t i None s' r ==> r
+let base_case' (#input #state: Type) (t: system input state bool): prop =
+  forall (i: input) (s: state) (s': state) (r: bool).
+    t.init s ==> t.step i s s' r ==> r
 
-let step_case (#input #state: Type) (t: stepfun input state prop): prop =
-  forall (i0 i1: input) (s0: option state) (s1 s2: state) (r0 r1: prop).
-    t i0 s0 s1 r0 ==> r0 ==>
-    t i1 (Some s1) s2 r1 ==> r1
+let step_case' (#input #state: Type) (t: system input state bool): prop =
+  forall (i0 i1: input) (s0: state) (s1 s2: state) (r0 r1: bool).
+    t.step i0 s0 s1 r0 ==> r0 ==>
+    t.step i1 s1 s2 r1 ==> r1
+
+let base_case (#input #state: Type) (t: system input state prop): prop =
+  forall (i: input) (s: state) (s': state) (r: prop).
+    t.init s ==> t.step i s s' r ==> r
+
+let step_case (#input #state: Type) (t: system input state prop): prop =
+  forall (i0 i1: input) (s0: state) (s1 s2: state) (r0 r1: prop).
+    t.step i0 s0 s1 r0 ==> r0 ==>
+    t.step i1 s1 s2 r1 ==> r1
 
 let induct1 (#input #state: Type)
-  (t: stepfun input state prop): prop =
+  (t: system input state prop): prop =
     base_case t /\ step_case t
 
 let rec induct1_sound (#len: nat) (#input #state: Type)
-  (t: stepfun input state prop)
+  (t: system input state prop)
   (inputs: C.vector input len)
   (props: C.vector prop len)
-  (s': option state):
+  (s': state):
     Lemma
-        (requires system_stepn' t inputs props s' /\ induct1 t)
+        (requires system_stepn t inputs props s' /\ induct1 t)
         (ensures prop_for_all props) =
  match inputs, props with
  | [], [] -> ()
  | [i], [p] -> ()
  | i1 :: i0 :: is, p1 :: p0 :: ps ->
    assert (len >= 2);
-   eliminate exists (s0: option state) (s1: state).
-     system_stepn' #(len - 2) t is ps s0 /\
-     t i0 s0 s1 p0
+   eliminate exists (s0: state) (s1: state).
+     system_stepn #(len - 2) t is ps s0 /\
+     t.step i0 s0 s1 p0
    returns prop_for_all props
    with h.
-     induct1_sound #(len - 1) t (i0 :: is) (p0 :: ps) (Some s1)
+     induct1_sound #(len - 1) t (i0 :: is) (p0 :: ps) s1
 
-let bmc2 (#input #state: Type) (t: stepfun input state prop): prop =
-  forall (i1 i2: input) (s1 s2: state) (r1 r2: prop).
-    t i1 None s1 r1 ==>
-    t i2 (Some s1) s2 r2 ==>
+let bmc2' (#input #state: Type) (t: system input state bool): prop =
+  forall (i1 i2: input) (s0 s1 s2: state) (r1 r2: bool).
+    t.init s0 ==>
+    t.step i1 s0 s1 r1 ==>
+    t.step i2 s1 s2 r2 ==>
+    r2
+
+let bmc2 (#input #state: Type) (t: system input state prop): prop =
+  forall (i1 i2: input) (s0 s1 s2: state) (r1 r2: prop).
+    t.init s0 ==>
+    t.step i1 s0 s1 r1 ==>
+    t.step i2 s1 s2 r2 ==>
     r2
 
 open Pipit.Exp.Base
@@ -78,8 +95,8 @@ let induct1_exp (#vars: nat)
   introduce forall (len: nat) (inputs: C.vector (C.row vars) len) (vs: C.vector bool len) (hBS: bigstep (C.Table inputs) e vs). List.Tot.for_all (fun r -> r) vs
   with
   begin
-    system_eval_complete' e (C.Table inputs) vs hBS;
-    eliminate exists (s': option (state_of_exp e)). system_stepn' (system_of_exp e vars) inputs vs s'
+    system_eval_complete e (C.Table inputs) vs hBS;
+    eliminate exists (s': (state_of_exp e)). system_stepn (system_of_exp e vars) inputs vs s'
     returns _
     with hEx.
     begin
