src/Pipit.Check.Example.Manual.fst
@@ -1,0 +1,56 @@
+module Pipit.Check.Example.Manual
+
+open Pipit.System.Base
+open Pipit.System.Ind
+
+module T = FStar.Tactics
+
+// sofar e => once e
+let example0_manual: system bool (bool * bool) bool =
+  { init = (fun (sofar, once) -> (sofar = true) /\ (once = false));
+    step = (fun i (sofar, once) (sofar', once') r ->
+                sofar' = (sofar && i) /\
+                once' = (once || i) /\
+                r == (if sofar' then once' else true)
+      ) }
+
+let example0_manual' = system_map prop_of_bool example0_manual
+
+let example0_ok_base (_: unit): Lemma (ensures base_case' example0_manual) =
+  ()
+
+let example0_ok_step (_: unit):
+  Lemma (ensures step_case' example0_manual) =
+  assert (step_case' example0_manual) by (T.compute (); T.dump "step_case");
+  ()
+
+let example0_ok_induct (_: unit):
+  Lemma (ensures induct1 example0_manual') =
+  // example0_ok_base ();
+  // example0_ok_step ();
+  ()
+
+
+
+// the encoding from translating the expression has more existentials, so try adding them
+// sofar e => once e
+let exampleX_manual: system bool (bool * bool) bool =
+  { init = (fun (sofar, once) -> (sofar = true) /\ (once = false));
+    step = (fun i (sofar, once) (sofar', once') r ->
+                exists ss oo.
+                ss = (sofar && i) /\
+                oo = (once || i) /\
+                sofar' = ss /\
+                once' = oo /\
+                r == (if ss then oo else true)
+      ) }
+
+let exampleX_manual' = system_map prop_of_bool example0_manual
+
+let exampleX_ok_base (_: unit): Lemma (ensures base_case' exampleX_manual) =
+  ()
+
+let exampleX_ok_step (_: unit):
+  Lemma (ensures step_case' exampleX_manual) =
+  assert (step_case' exampleX_manual) by (T.compute (); T.dump "step_case");
+  ()
