src/Pipit.System.ExpX.fst
@@ -1,0 +1,151 @@
+(* Transition systems *)
+module Pipit.System.ExpX
+
+open Pipit.System.Base
+
+open Pipit.Exp.Base
+open Pipit.Exp.Bigstep
+open Pipit.Exp.Causality
+
+module C = Pipit.Context
+
+let rec state_of_exp (e: exp): Type =
+  match e with
+  | XVal v -> unit
+  | XVar x -> unit
+  | XPrim2 p e1 e2 -> state_of_exp e1 * state_of_exp e2
+  | XPre e1 -> state_of_exp e1 * value
+  | XThen e1 e2 -> bool * state_of_exp e2
+  | XMu e1 -> state_of_exp e1
+
+let rec oracle_of_exp (e: exp): Type =
+  match e with
+  | XVal v -> unit
+  | XVar x -> unit
+  | XPrim2 p e1 e2 -> value * value * oracle_of_exp e1 * oracle_of_exp e2
+  | XPre e1 -> oracle_of_exp e1
+  | XThen e1 e2 -> state_of_exp e1 * state_of_exp e1 * value * oracle_of_exp e1 * oracle_of_exp e2
+  | XMu e1 -> oracle_of_exp e1
+
+(* An system with "oracles", which let us draw out the quantifiers to the top level *)
+let osystem (input: Type) (oracle: Type) (state: Type) (result: Type) = system (input * oracle) state result
+
+(* A system we get from translating an expression *)
+let xsystem (e: exp) (vars: nat { wf e vars }) = osystem (C.row vars) (oracle_of_exp e) (state_of_exp e) value
+
+let osystem_input (#input #oracle: Type): osystem input oracle unit input =
+  { init = (fun s -> True);
+    step = (fun (i, o) s s' r -> r == i) }
+
+let osystem_index (vars: nat) (x: nat { x < vars }):
+       osystem (C.row vars) unit unit value =
+  { init = (fun _ -> True);
+    step = (fun (i, o) s s' r ->
+      r == C.row_index i x)
+  }
+
+let osystem_map2 (#input #oracle1 #oracle2 #state1 #state2 #value1 #value2 #result: Type) (f: value1 -> value2 -> result)
+  (t1: osystem input oracle1 state1 value1)
+  (t2: osystem input oracle2 state2 value2):
+       osystem input (value1 * value2 * oracle1 * oracle2) (state1 * state2) result =
+   {
+    init = (fun (s1, s2) -> t1.init s1 /\ t2.init s2);
+    step = (fun (i, (r1, r2, o1, o2)) (s1, s2) (s1', s2') r ->
+               t1.step (i, o1) s1 s1' r1 /\
+               t2.step (i, o2) s2 s2' r2 /\
+               r == f r1 r2)
+  }
+
+let osystem_pre (#input #oracle1 #state1 #v: Type) (init: v)
+  (t1: osystem input oracle1 state1 v):
+       osystem input oracle1 (state1 * v) v =
+  { init = (fun (s1, v) -> t1.init s1 /\ v == init);
+    step = (fun i (s1, v) (s1', v') r ->
+      t1.step i s1 s1' v' /\ r == v)
+  }
+
+let osystem_then (#input #oracle1 #oracle2 #state1 #state2 #v: Type)
+  (t1: osystem input oracle1 state1 v)
+  (t2: osystem input oracle2 state2 v):
+       osystem input (state1 * state1 * v * oracle1 * oracle2) (bool * state2) v =
+  { init = (fun (init,s2) -> init = true /\ t2.init s2);
+    step = (fun (i, (s1, s1', r', o1, o2)) (init, s2) (init', s2') r ->
+     if init
+     then t1.init s1 /\ t1.step (i, o1) s1 s1' r /\ t2.step (i, o2) s2 s2' r'
+     else init = false /\ t2.step (i, o2) s2 s2' r)
+  }
+
+let osystem_mu (#input #input' #oracle #state1 #v: Type)
+  (extend: input -> v -> input')
+  (t1: osystem input' oracle state1 v):
+       osystem input  oracle state1 v =
+  { init = t1.init;
+    step = (fun (i, o) s s' r -> t1.step (extend i r, o) s s' r)
+  }
+
+irreducible let unfold_attr = ()
+
+[@@unfold_attr]
+let rec osystem_of_exp (e: exp) (vars: nat { wf e vars }):
+    xsystem e vars =
+  match e with
+  | XVal v -> system_const v
+  | XVar x -> osystem_index vars x
+  | XPrim2 p e1 e2 ->
+    osystem_map2 (eval_prim2 p) (osystem_of_exp e1 vars) (osystem_of_exp e2 vars)
+  | XPre e1 ->
+    osystem_pre xpre_init (osystem_of_exp e1 vars)
+  | XThen e1 e2 ->
+    osystem_then (osystem_of_exp e1 vars) (osystem_of_exp e2 vars)
+  | XMu e1 ->
+    let t = osystem_of_exp e1 (vars + 1) in
+    osystem_mu #(C.row vars) #(C.row (vars + 1)) (fun i v -> C.row_append (C.row1 v) i) t
+
+// let rec osystem_of_exp_init (e: exp) (vars: nat { wf e vars }) (s: state_of_exp e): prop =
+//   match e with
+//   | XVal v -> True
+//   | XVar x -> True
+//   | XPrim2 p e1 e2 ->
+//     let ss = s <: state_of_exp e1 * state_of_exp e2 in
+//     osystem_of_exp_init e1 vars (fst ss) /\
+//     osystem_of_exp_init e2 vars (snd ss)
+//   | XPre e1 ->
+//     let ss = s <: state_of_exp e1 * value in
+//     osystem_of_exp_init e1 vars (fst ss) /\ (snd ss) = xpre_init
+//   | XThen e1 e2 ->
+//     osystem_then (osystem_of_exp e1 vars) (osystem_of_exp e2 vars)
+//   | XMu e1 ->
+//     let t = osystem_of_exp e1 (vars + 1) in
+//     osystem_mu #(C.row vars) #(C.row (vars + 1)) (fun i v -> C.row_append (C.row1 v) i) t
+
+
+module Ck = Pipit.Check.Example
+module T = FStar.Tactics
+
+open Pipit.System.Ind
+
+
+
+let wf_ (): wf_: nat { wf (Ck.example0_ok Ck.x0) wf_ } = 1
+let example0_t = osystem_of_exp (Ck.example0_ok Ck.x0) 1
+
+let example0_ok_base (): Lemma (ensures base_case' example0_t) =
+
+  assert (base_case' example0_t) by (
+    T.compute ();
+    // let _ = T.forall_intros () in
+    T.norm [delta_attr [`%unfold_attr]];
+    T.whnf ();
+    T.unfold_def (`osystem_of_exp);
+    // T.l_revert ();
+    // T.revert ();
+    // T.implies_intro ();
+    // T.forall_intro ();
+    T.dump "wbase_case"
+  );
+
+  admit ()
+
+let example0_ok_step (): Lemma (ensures step_case' example0_t) =
+  assert (step_case' example0_t) by (T.compute (); T.dump "step_case");
+  ()
